\subsection{First consequences} \ 

\begin{dc}\label{c6}%
If $\vdash\metavariable{A}\implies\metavariable{B}$ and $\vdash\metavariable{B}\implies\metavariable{C}$,
then $\vdash\metavariable{A}\implies\metavariable{C}$.
\end{dc}

\begin{pf}
\item\label{dc6:1} $\vdash(\metavariable{A}\implies\metavariable{B})$
  by hypothesis
\item\label{dc6:2} $\vdash(\metavariable{B}\implies\metavariable{C})$
  by hypothesis
\item\label{dc6:3} $\vdash(\metavariable{B}\implies\metavariable{C})\implies((\neg\metavariable{A}\lor\metavariable{B})\implies(\neg\metavariable{A}\lor\metavariable{C}))$
  by \ref{axiom:s4}$(\metavariable{B},\metavariable{C},\neg\metavariable{A})$.
\item\label{dc6:4} $\vdash((\neg\metavariable{A}\lor\metavariable{B})\implies(\neg\metavariable{A}\lor\metavariable{C}))$
  by MP(\ref{dc6:3},\ref{dc6:2})
\item\label{dc6:5} $\vdash(\neg\metavariable{A}\lor\metavariable{B})$
  by \ref{unfold-implies}(\ref{dc6:1})
\item\label{dc6:6} $\vdash(\neg\metavariable{A}\lor\metavariable{C})$ by MP(\ref{dc6:4},\ref{dc6:5}).
\item\label{dc6:7} $\vdash(\metavariable{A}\implies\metavariable{C})$ by \ref{fold-implies}(\ref{dc6:6})
\end{pf}

\begin{dc}\label{c7}%
$\vdash\metavariable{B}\implies(\metavariable{A}\lor\metavariable{B})$.
\end{dc}

\begin{pf}
\item\label{dc7:1} $\vdash\metavariable{B}\implies(\metavariable{B}\lor\metavariable{A})$
  by $\ref{axiom:s2}(\metavariable{B},\metavariable{A})$
\item\label{dc7:2} $\vdash(\metavariable{B}\lor\metavariable{A})\implies(\metavariable{A}\lor\metavariable{B})$
  by $\ref{axiom:s3}(\metavariable{B},\metavariable{A})$
\item $\vdash\metavariable{B}\implies(\metavariable{A}\lor\metavariable{B})$
  by \ref{c6}(\ref{dc7:1}, \ref{dc7:2})
\end{pf}

\begin{dc}\label{c8}%
$\vdash\metavariable{A}\implies\metavariable{A}$
\end{dc}

\begin{pf}
\item\label{dc8:1} $\vdash\metavariable{A}\implies(\metavariable{A}\lor\metavariable{A})$
  by \ref{axiom:s2}($\metavariable{A}$, $\metavariable{A}$)
\item\label{dc8:2} $\vdash(\metavariable{A}\lor\metavariable{A})\implies\metavariable{A}$
  by \ref{axiom:s1}($\metavariable{A}$)
\item $\vdash\metavariable{A}\implies\metavariable{A}$ by
  \ref{c6}(\ref{dc8:1}, \ref{dc8:2})
\end{pf}

\begin{dc}\label{c9}%
If $\vdash\metavariable{B}$, then for any proposition $\metavariable{A}$
we have $\vdash\metavariable{A}\implies\metavariable{B}$.
\end{dc}

\begin{pf}
\item\label{dc9:1} $\vdash\metavariable{B}$ by hypothesis
\item\label{dc9:2} $\vdash\metavariable{B}\implies(\neg\metavariable{A}\lor\metavariable{B})$
  by \ref{c7}($\neg{\metavariable{A}}$, $\metavariable{B}$)
\item\label{dc9:3} $\vdash\neg\metavariable{A}\lor\metavariable{B}$ by
  MP(\ref{dc9:1}, \ref{dc9:2})
\item $\vdash\metavariable{A}\implies\metavariable{B}$ by \ref{fold-implies}(\ref{dc9:3})
\end{pf}

\begin{dc}\label{c10}%
$\vdash\metavariable{A}\lor\neg\metavariable{A}$
\end{dc}
\begin{pf}
\item\label{dc10:1} $\vdash\metavariable{A}\implies\metavariable{A}$
  by \ref{c8}($\metavariable{A}$)
\item\label{dc10:2} $\vdash\neg\metavariable{A}\lor\metavariable{A}$
  by \ref{unfold-implies}(\ref{dc10:1})
\item\label{dc10:3} $\vdash((\neg\metavariable{A})\lor\metavariable{A})\implies(\metavariable{A}\lor\neg\metavariable{A})$
  by \ref{axiom:s3}($\neg\metavariable{A}$, $\metavariable{A}$)
\item $\vdash\metavariable{A}\lor\neg\metavariable{A}$ by
  MP(\ref{dc10:3}, \ref{dc10:2})
\end{pf}

\begin{dc}\label{c11}%
$\vdash\metavariable{A}\implies(\neg\neg\metavariable{A})$
\end{dc}

\begin{pf}
\item\label{dc11:1} $\vdash(\neg\metavariable{A})\lor(\neg\neg\metavariable{A})$
  by \ref{c10}($\metavariable{A}$)
\item $\vdash\metavariable{A}\implies\neg\neg\metavariable{A}$
  by \ref{fold-implies}(\ref{dc11:1})
\end{pf}

\begin{dc}\label{c12}%
$\vdash(\metavariable{A}\implies\metavariable{B})\implies((\neg\metavariable{B})\implies(\neg\metavariable{A}))$
\end{dc}

\begin{pf}
\item\label{dc12:1} $\vdash\metavariable{B}\implies\neg\neg\metavariable{B}$
  by \ref{c11}($\metavariable{B}$)
\item\label{dc12:2} $\vdash(\metavariable{B}\implies\neg\neg\metavariable{B})\implies((\neg\metavariable{A}\lor\metavariable{B})\implies(\neg\metavariable{A}\lor\neg\neg\metavariable{B}))$
  by \ref{axiom:s4}($\metavariable{B}$, $\neg\neg\metavariable{B}$, $\neg\metavariable{A}$)
\item\label{dc12:3} $\vdash(\neg\metavariable{A}\lor\metavariable{B})\implies(\neg\metavariable{A}\lor\neg\neg\metavariable{B})$
  by MP(\ref{dc12:2}, \ref{dc12:1})
\item\label{dc12:4} $\vdash(\neg\metavariable{A}\lor\neg\neg\metavariable{B})\implies(\neg\neg\metavariable{B}\lor\neg\metavariable{A})$
  by \ref{axiom:s3}($\neg\metavariable{A}$, $\neg\neg\metavariable{B}$)
\item\label{dc12:5} $\vdash(\neg\metavariable{A}\lor\metavariable{B})\implies(\neg\neg\metavariable{B}\lor\neg\metavariable{A})$
  by \ref{c6}(\ref{dc12:3}, \ref{dc12:4})
\item\label{dc12:6} $\vdash(\metavariable{A}\implies\metavariable{B})\implies(\neg\metavariable{A}\lor\metavariable{B})$
  by \ref{syn:tautology:implies-to-lor}($\metavariable{A}$, $\metavariable{B}$)
\item\label{dc12:7} $\vdash(\metavariable{A}\implies\metavariable{B})\implies(\neg\neg\metavariable{B}\lor\neg\metavariable{A})$
  by \ref{c6}(\ref{dc12:6}, \ref{dc12:5})
\item\label{dc12:8} $\vdash(\neg\neg\metavariable{B}\lor\neg\metavariable{A})\implies(\neg\metavariable{B}\implies\neg\metavariable{A})$
  by \ref{syn:tautology:implies-to-lor}($\neg\metavariable{B}$, $\neg\metavariable{A}$)
\item $\vdash(\metavariable{A}\implies\metavariable{B})\implies(\neg\metavariable{B}\implies\neg\metavariable{A})$
  by \ref{c6}(\ref{dc12:7}, \ref{dc12:8})
\end{pf}

\begin{dc}\label{c13}%
If $\vdash\metavariable{A}\implies\metavariable{B}$,
then $\vdash(\metavariable{B}\implies\metavariable{C})\implies(\metavariable{A}\implies\metavariable{C})$
\end{dc}

\begin{pf}
\item\label{dc13:1} $\vdash\metavariable{A}\implies\metavariable{B}$ by hypothesis
\item\label{dc13:2} $\vdash(\metavariable{A}\implies\metavariable{B})\implies(\neg\metavariable{B}\implies\neg\metavariable{A})$
  by \ref{c12}($\metavariable{A}$, $\metavariable{B}$)
\item\label{dc13:3} $\vdash\neg\metavariable{B}\implies\neg\metavariable{A}$
  by MP(\ref{dc13:2}, \ref{dc13:1})
\item\label{dc13:4} $\vdash(\neg\metavariable{B}\implies\neg\metavariable{A})\implies((\metavariable{C}\lor\neg\metavariable{B})\implies(\metavariable{C}\lor\neg\metavariable{A}))$
  by \ref{axiom:s4}($\neg\metavariable{B}$, $\neg\metavariable{A}$, $\metavariable{C}$)
\item\label{dc13:5} $\vdash(\metavariable{C}\lor\neg\metavariable{B})\implies(\metavariable{C}\lor\neg\metavariable{A})$
  by MP(\ref{dc13:4}, \ref{dc13:3})
\item\label{dc13:6} $\vdash(\metavariable{B}\implies\metavariable{C})\implies(\metavariable{C}\lor\neg\metavariable{B})$
  by \ref{c6}(\ref{syn:tautology:implies-to-lor}($\metavariable{B}$, $\metavariable{C}$),
  \ref{axiom:s3}($\metavariable{C}$, $\neg\metavariable{B}$))
\item\label{dc13:7} $\vdash(\metavariable{B}\implies\metavariable{C})\implies(\metavariable{C}\lor\neg\metavariable{A})$
  by \ref{c6}(\ref{dc13:6}, \ref{dc13:5})
\item\label{dc13:8} $\vdash(\metavariable{C}\lor\neg\metavariable{A})\implies(\metavariable{A}\implies\metavariable{C})$
  by \ref{c6}(\ref{axiom:s3}($\metavariable{C}$, $\neg\metavariable{A}$),
  \ref{syn:tautology:lor-to-implies}($\metavariable{A}$, $\metavariable{C}$))
\item $\vdash(\metavariable{B}\implies\metavariable{C})\implies(\metavariable{A}\implies\metavariable{C})$
  by \ref{c6}(\ref{dc13:7}, \ref{dc13:8})
\end{pf}

\begin{theorem}\label{thm:3-2-1}%
If $\vdash\metavariable{A}\implies\metavariable{B}$, then $\vdash\metavariable{A}\lor\metavariable{B}\implies\metavariable{B}$.
\end{theorem}

\begin{pf}
\item\label{step:3-2-1:1} $\vdash\metavariable{A}\implies\metavariable{B}$
  by hypothesis
\item\label{step:3-2-1:2} $\vdash(\metavariable{A}\implies\metavariable{B})\implies((\metavariable{B}\lor\metavariable{A})\implies(\metavariable{B}\lor\metavariable{B}))$
by \ref{axiom:s4}($\metavariable{A}$, $\metavariable{B}$, $\metavariable{B}$)
\item\label{step:3-2-1:3} $\vdash\metavariable{A}\lor\metavariable{B}\implies\metavariable{B}\lor\metavariable{A}$
by \ref{axiom:s3}($\metavariable{A}$, $\metavariable{B}$)
\item\label{step:3-2-1:4} $\vdash\metavariable{B}\lor\metavariable{A}\implies\metavariable{B}\lor\metavariable{B}$
by MP(\ref{step:3-2-1:2}, \ref{step:3-2-1:1})
\item\label{step:3-2-1:5} $\vdash\metavariable{A}\lor\metavariable{B}\implies\metavariable{B}\lor\metavariable{B}$
by \ref{c6}(\ref{step:3-2-1:3}, \ref{step:3-2-1:4})
\item\label{step:3-2-1:6} $\vdash\metavariable{B}\lor\metavariable{B}\implies\metavariable{B}$
  by \ref{axiom:s1}($\metavariable{B}$)
\item\label{step:3-2-1:7} $\vdash\metavariable{A}\lor\metavariable{B}\implies\metavariable{B}$
  by \ref{c6}(\ref{step:3-2-1:5}, \ref{step:3-2-1:6})
\end{pf}

\begin{theorem}\label{thm:3-2-2}%
If $\vdash\metavariable{A}\implies\metavariable{C}$
and $\vdash\metavariable{B}\implies\metavariable{C}$,
then $\vdash\metavariable{A}\lor\metavariable{B}\implies\metavariable{C}$.
\end{theorem}

\begin{pf}
\item\label{step:3-2-2:1} $\vdash\metavariable{A}\implies\metavariable{C}$
  by hypothesis
\item\label{step:3-2-2:2} $\vdash\metavariable{B}\implies\metavariable{C}$
  by hypothesis
\item\label{step:3-2-2:3} $\vdash(\metavariable{B}\implies\metavariable{C})\implies((\metavariable{A}\lor\metavariable{B})\implies(\metavariable{A}\lor\metavariable{C}))$
  by \ref{axiom:s4}($\metavariable{B}$, $\metavariable{C}$, $\metavariable{A}$)
\item\label{step:3-2-2:4} $\vdash\metavariable{A}\lor\metavariable{B}\implies\metavariable{A}\lor\metavariable{C}$
  by MP(\ref{step:3-2-2:3}, \ref{step:3-2-2:2})
\item\label{step:3-2-2:5} $\vdash\metavariable{A}\lor\metavariable{C}\implies\metavariable{C}$
  by Thm\ref{thm:3-2-1}(\ref{step:3-2-2:1})
\item\label{step:3-2-2:6} $\vdash\metavariable{A}\lor\metavariable{B}\implies\metavariable{C}$
  by \ref{c6}(\ref{step:3-2-2:4}, \ref{step:3-2-2:5})
\end{pf}
