\subsection{Conjunction}

\begin{definition}
Let $\metavariable{A}$ and $\metavariable{B}$ be assemblies. Then $\neg((\neg\metavariable{A})\lor(\neg\metavariable{B}))$
is denoted ``$\metavariable{A}\land\metavariable{B}$'' (or
``$\metavariable{A}$ and $\metavariable{B}$'').
\end{definition}

\begin{cs}\label{cs6}%
Let $\metavariable{A}$, $\metavariable{B}$, $\metavariable{T}$ be
assemblies and let $\metavariable{x}$ be a letter. Then $(\metavariable{T}\mid\metavariable{x})(\metavariable{A}\land\metavariable{B})$
is identical to $\metavariable{A}'\land\metavariable{B}'$ where
$\metavariable{A}'$ is identical to $(\metavariable{T}\mid\metavariable{x})\metavariable{A}$
and $\metavariable{B}'$ is identical to $(\metavariable{T}\mid\metavariable{x})\metavariable{B}$.
\end{cs}

\begin{proof}
This is a direct consequence of \ref{cs5}
\begin{subequations}
\begin{align}
(\metavariable{T}\mid\metavariable{x})\metavariable{A}\land\metavariable{B}
&=(\metavariable{T}\mid\metavariable{x})\neg((\neg\metavariable{A})\lor(\neg\metavariable{B}))\\
&=\neg[(\metavariable{T}\mid\metavariable{x})((\neg\metavariable{A})\lor(\neg\metavariable{B}))]\\
&=\neg([(\metavariable{T}\mid\metavariable{x})(\neg\metavariable{A})]\lor[(\metavariable{T}\mid\metavariable{x})(\neg\metavariable{B})])\\
&=\neg([(\neg(\metavariable{T}\mid\metavariable{x})\metavariable{A})]\lor[(\neg(\metavariable{T}\mid\metavariable{x})\metavariable{B})])\\
&=\metavariable{A}'\land\metavariable{B}',
\end{align}
\end{subequations}
as desired.
\end{proof}

\begin{cf}\label{cf9}%
If $\metavariable{A}$ and $\metavariable{B}$ are relations in $\theory{T}$,
then $\metavariable{A}\land\metavariable{B}$ is a relation in $\theory{T}$
(called the \define{Conjunction} of $\metavariable{A}$ and $\metavariable{B}$).
\end{cf}

This follows from \ref{cf1} and \ref{cf2}.

\begin{dc}\label{c20}%
If $\vdash\metavariable{A}$ and $\vdash\metavariable{B}$, then $\vdash\metavariable{A}\land\metavariable{B}$.
\end{dc}
I formalize Bourbaki's proof, there is almost certainly a more optimal proof.
\begin{pf}
\item\label{step:c20:1} $\vdash\metavariable{A}$ by hypothesis
\item\label{step:c20:2} $\vdash\metavariable{B}$ by hypothesis
\item\label{step:c20:3} $\neg(\metavariable{A}\land\metavariable{B})\vdash\neg\neg((\neg\metavariable{A})\lor(\neg\metavariable{B}))$
by assumption, definition of conjunction
\item\label{step:c20:4} $\neg(\metavariable{A}\land\metavariable{B})\vdash(\neg\neg((\neg\metavariable{A})\lor(\neg\metavariable{B})))\implies((\neg\metavariable{A})\lor(\neg\metavariable{B}))$
by \ref{c16}($(\neg\metavariable{A})\lor(\neg\metavariable{B})$)
\item\label{step:c20:5} $\neg(\metavariable{A}\land\metavariable{B})\vdash(\neg\metavariable{A})\lor(\neg\metavariable{B})$
by MP(\ref{step:c20:4}, \ref{step:c20:3})
\item\label{step:c20:6} $\neg(\metavariable{A}\land\metavariable{B})\vdash((\neg\metavariable{A})\lor(\neg\metavariable{B}))\implies(\metavariable{A}\implies\neg\metavariable{B})$
by \ref{syn:tautology:lor-to-implies}($\metavariable{A}$, $\neg\metavariable{B}$)
\item\label{step:c20:7} $\neg(\metavariable{A}\land\metavariable{B})\vdash\metavariable{A}\implies\neg\metavariable{B}$
by MP(\ref{step:c20:6}, \ref{step:c20:5})
\item\label{step:c20:8} $\neg(\metavariable{A}\land\metavariable{B})\vdash\metavariable{A}$
by weakening(\ref{step:c20:1})
\item\label{step:c20:9} $\neg(\metavariable{A}\land\metavariable{B})\vdash\neg\metavariable{B}$
by MP(\ref{step:c20:7}, \ref{step:c20:8})
\item\label{step:c20:10} $\neg(\metavariable{A}\land\metavariable{B})\vdash\metavariable{B}$
by weakening(\ref{step:c20:2})
\item\label{step:c20:11} $\vdash\metavariable{A}\land\metavariable{B}$
by \ref{c15}(\ref{step:c20:10}, \ref{step:c20:9}).
\end{pf}

\begin{dc}\label{c21}%
We have the following results for any formulas
$\metavariable{A}$ and $\metavariable{B}$:
\begin{enumerate}
\item $\vdash(\metavariable{A}\land\metavariable{B})\implies\metavariable{A}$
\item $\vdash(\metavariable{A}\land\metavariable{B})\implies\metavariable{B}$
\end{enumerate}
\end{dc}

\begin{enumerate}
\item 
\begin{pf}
\item\label{step:c21:1} $\vdash\phantom{(}(\neg\metavariable{A})\implies\neg(\metavariable{A}\land\metavariable{B})$
by \ref{axiom:s3}($\neg\metavariable{A}$, $\neg\metavariable{B}$),
definition of conjunction
\item\label{step:c21:2} $\vdash((\neg\metavariable{A})\implies\neg(\metavariable{A}\land\metavariable{B}))\implies(\metavariable{A}\land\metavariable{B}\implies\metavariable{A})$
by \ref{c17}($\metavariable{A}\land\metavariable{B}$, $\metavariable{A}$)
\item\label{step:c21:3} $\vdash\metavariable{A}\land\metavariable{B}\implies\metavariable{A}$
by MP(\ref{step:c21:2}, \ref{step:c21:1}).
\end{pf}
\item 
\begin{pf}
\item\label{step:c21:2:1} $\vdash\phantom{(}\neg\metavariable{B}\implies\neg\metavariable{A}\lor\neg\metavariable{B}$
by \ref{c7}($\neg\metavariable{A}$, $\neg\metavariable{B}$)
\item\label{step:c21:2:2} $\vdash(\neg\metavariable{B}\implies\neg\metavariable{A}\lor\neg\metavariable{B})\implies(\metavariable{A}\land\metavariable{B}\implies\metavariable{B})$
by \ref{c17}($\metavariable{A}\land\metavariable{B}$, $\metavariable{B}$),
definition of conjunction
\item\label{step:c21:2:3} $\vdash\metavariable{A}\land\metavariable{B}\implies\metavariable{B}$
by MP(\ref{step:c21:2:2}, \ref{step:c21:2:1}).
\end{pf}
\end{enumerate}
