\subsection{Equivalence}

\begin{definition}
Let $\metavariable{A}$ and $\metavariable{B}$ be assemblies. The
assembly
$(\metavariable{A}\implies\metavariable{B})\land(\metavariable{B}\implies\metavariable{A})$
will be denoted by ``$\metavariable{A}\iff\metavariable{B}$''.
\end{definition}

\begin{cs}\label{cs7}%
Let $\metavariable{A}$, $\metavariable{B}$, $\metavariable{T}$ be
assemblies, let $\metavariable{x}$ be a letter. Then $(\metavariable{T}\mid\metavariable{x})(\metavariable{A}\iff\metavariable{B})$
is identical to $\metavariable{A}'\iff\metavariable{B}'$ where
$\metavariable{A}'$ is $(\metavariable{T}\mid\metavariable{x})\metavariable{A}$
and $\metavariable{B}'$ is $(\metavariable{T}\mid\metavariable{x})\metavariable{B}$.
\end{cs}

\begin{proof}[Proof sketch]
This follows from \ref{cs5} and \ref{cs6}.
\end{proof}

\begin{cf}\label{cf10}%
If $\metavariable{A}$ and $\metavariable{B}$ are relations in $\theory{T}$,
then $\metavariable{A}\iff\metavariable{B}$ is a relation in $\theory{T}$.
\end{cf}

\begin{proof}[Proof sketch]
This follows from \ref{cf5} and \ref{cf9}.
\end{proof}

\begin{dc}\label{c22}%
The biconditional is an equivalence relation. Bourbaki skips
reflexivity, which I included as item (0).
\begin{enumerate}[start=0]
\item $\vdash\metavariable{A}\iff\metavariable{A}$
\item If $\vdash\metavariable{A}\iff\metavariable{B}$, then $\vdash\metavariable{B}\iff\metavariable{A}$
\item If $\vdash\metavariable{A}\iff\metavariable{B}$ and $\vdash\metavariable{B}\iff\metavariable{C}$,
then $\vdash\metavariable{A}\iff\metavariable{C}$.
\end{enumerate}
\end{dc}

\begin{proof}[Proof sketch]
(0) follows from \ref{c20}(\ref{c8}($\metavariable{A}$), \ref{c8}($\metavariable{A}$)).

(1) and (2) follows from \ref{c20} and \ref{c21}.
\end{proof}

At this point, it's painfully clear that Bourbaki is ``running out of steam'',
because the proofs are increasingly sketch for \ref{c22}, and completely
omitted afterwards. The remaining deductive criteria given are
enumerated faithfully (i.e., Bourbaki just gives a list of results).

\begin{dc}\label{c23}%
Let $\metavariable{A}$ and $\metavariable{B}$ be equivalent relations
(i.e., $\vdash\metavariable{A}\iff\metavariable{B}$), let
$\metavariable{C}$ be an arbitrary relation. Then:
\begin{enumerate}
\item $\vdash(\neg\metavariable{A})\iff(\neg\metavariable{B})$
\item $\vdash(\metavariable{A}\implies\metavariable{C})\iff(\metavariable{B}\implies\metavariable{C})$
\item $\vdash(\metavariable{A}\land\metavariable{C})\iff(\metavariable{B}\land\metavariable{C})$
\item $\vdash(\metavariable{C}\implies\metavariable{A})\iff(\metavariable{C}\implies\metavariable{B})$
\item $\vdash(\metavariable{A}\lor\metavariable{C})\iff(\metavariable{B}\lor\metavariable{C})$
\end{enumerate}
\end{dc}

\begin{dc}\label{c24}%
Let $\metavariable{A}$, $\metavariable{B}$, $\metavariable{C}$ be
arbitrary relations. Then:
\begin{enumerate}
\item $\vdash(\neg\neg\metavariable{A})\iff\metavariable{A}$ [hint: \ref{c11}($\metavariable{A}$),
\ref{c16}($\metavariable{A}$)]
\item $\vdash(\metavariable{A}\implies\metavariable{B})\iff(\neg\metavariable{B}\implies\neg\metavariable{A})$
[hint: \ref{c12}($\metavariable{A}$, $\metavariable{B}$),
  \ref{c17}($\metavariable{A}$, $\metavariable{B}$)]
\item $\vdash(\metavariable{A}\land\metavariable{A})\iff\metavariable{A}$
\item $\vdash(\metavariable{A}\land\metavariable{B})\iff(\metavariable{B}\land\metavariable{A})$
\item $\vdash\metavariable{A}\land(\metavariable{B}\land\metavariable{C})\iff(\metavariable{A}\land\metavariable{B})\land\metavariable{C}$
\item $\vdash(\metavariable{A}\lor\metavariable{B})\iff\neg((\neg\metavariable{A})\lor(\neg\metavariable{B}))$
\item $\vdash\metavariable{A}\lor\metavariable{A}\iff\metavariable{A}$
\item $\vdash\metavariable{A}\lor\metavariable{B}\iff\metavariable{B}\lor\metavariable{A}$
by \ref{axiom:s3}($\metavariable{A}$, $\metavariable{B}$) and \ref{axiom:s3}($\metavariable{B}$, $\metavariable{A}$)
\item $\vdash\metavariable{A}\lor(\metavariable{B}\lor\metavariable{C})\iff(\metavariable{A}\lor\metavariable{B})\lor\metavariable{C}$
\item $\vdash\metavariable{A}\land(\metavariable{B}\lor\metavariable{C})\iff(\metavariable{A}\land\metavariable{B})\lor(\metavariable{A}\land\metavariable{C})$
\item $\vdash\metavariable{A}\lor(\metavariable{B}\land\metavariable{C})\iff(\metavariable{A}\lor\metavariable{B})\land(\metavariable{A}\land\metavariable{C})$
\item $\vdash\metavariable{A}\land(\neg\metavariable{B})\iff\neg(\metavariable{A}\implies\metavariable{B})$
\item $\vdash\metavariable{A}\lor\metavariable{B}\iff((\neg\metavariable{A})\implies\metavariable{B})$
\end{enumerate}
\end{dc}

\begin{dc}\label{c25}%
Let $\metavariable{A}$ and $\metavariable{B}$ be any formulas. Then:
\begin{enumerate}
\item If $\vdash\metavariable{A}$, then $\vdash(\metavariable{A}\land\metavariable{B})\iff\metavariable{B}$.
\item If $\vdash\neg\metavariable{A}$, then $\vdash(\metavariable{A}\lor\metavariable{B})\iff\metavariable{B}$.
\end{enumerate}
\end{dc}
