\subsection{Properties of Quantified Theories}

\subsubsection{Reservation}
Bourbaki, for the rest of this section, considers $\theory{T}$ to be a
quantified theory. Further, the theory $\theory{T}_{0}$ consists of the
same signs as $\theory{T}$ but $\theory{T}_{0}$ has no explicit axioms
and only schemes \ref{axiom:s1} through \ref{axiom:s5}. Observe that
$\theory{T}$ is stronger (\S\ref{defn:stronger-theory}) than $\theory{T}_{0}$.

\begin{dc}\label{c29}%
Let $\metavariable{R}$ be a relation in $\theory{T}$, let
$\metavariable{x}$ be a letter. Then $\vdash\bigl(\neg(\exists\metavariable{x})\metavariable{R}\bigr)\iff\bigl((\forall\metavariable{x})\neg\metavariable{R}\bigr)$
\end{dc}

\begin{dc}\label{c30}%
Let $\metavariable{R}$ be a relation in $\theory{T}$, let
$\metavariable{T}$ be a term in $\theory{T}$, let $\metavariable{x}$ be
a letter. Then $\vdash(\forall\metavariable{x})\metavariable{R}\implies(\metavariable{T}\mid\metavariable{x})\metavariable{R}$.
\end{dc}

\begin{pf}
\item\label{step:c30:1}\Pf $\vdash(\metavariable{T}\mid\metavariable{x})\neg\metavariable{R}\implies(\tau_{\metavariable{x}}(\neg\metavariable{R})\mid\metavariable{x})\neg\metavariable{R}$
by \ref{axiom:s5}($\neg\metavariable{R}$, $\metavariable{T}$, $\metavariable{x}$)
\item\label{step:c30:2} $\vdash\neg(\metavariable{T}\mid\metavariable{x})\metavariable{R}\implies\neg(\tau_{\metavariable{x}}(\neg\metavariable{R})\mid\metavariable{x})\metavariable{R}$
by \ref{cs5}
\item\label{step:c30:3} $\vdash(\tau_{\metavariable{x}}(\neg\metavariable{R})\mid\metavariable{x})\metavariable{R}\implies(\metavariable{T}\mid\metavariable{x})\metavariable{R}$
  by contrapositive of \ref{step:c30:2}
\item\label{step:c30:4} $\vdash(\forall\metavariable{x})\metavariable{R}\implies(\tau_{\metavariable{x}}(\neg\metavariable{R})\mid\metavariable{x})\metavariable{R}$
  by \ref{c26}($\metavariable{R}$, $\metavariable{x}$)
\item\label{step:c30:5} $\vdash(\forall\metavariable{x})\metavariable{R}\implies(\metavariable{T}\mid\metavariable{x})\metavariable{R}$
  by \ref{c6}(\ref{step:c30:4}, \ref{step:c30:3})
\end{pf}

\begin{dc}\label{c31}%
Let $\metavariable{R}$ and $\metavariable{S}$ be relations in $\theory{T}$.
Let $\metavariable{x}$ be a variable (i.e., a letter which is not a
constant in $\theory{T}$). Then:
\begin{enumerate}
\item If $\vdash\metavariable{R}\implies\metavariable{S}$, then $\vdash(\forall\metavariable{x})\metavariable{R}\implies(\forall\metavariable{x})\metavariable{S}$
\item If $\vdash\metavariable{R}\implies\metavariable{S}$, then $\vdash(\exists\metavariable{x})\metavariable{R}\implies(\exists\metavariable{x})\metavariable{S}$
\item If $\vdash\metavariable{R}\iff\metavariable{S}$, then $\vdash(\forall\metavariable{x})\metavariable{R}\iff(\forall\metavariable{x})\metavariable{S}$
\item If $\vdash\metavariable{R}\iff\metavariable{S}$, then $\vdash(\exists\metavariable{x})\metavariable{R}\iff(\exists\metavariable{x})\metavariable{S}$
\end{enumerate}
\end{dc}
Observe that (3) follows from (1), and (4) follows from (2). Therefore
it suffices to prove only (1) and (2).
\begin{enumerate}
\item
\begin{pf}
\item\label{step:c31a:1}\Pf $\vdash\metavariable{R}\implies\metavariable{S}$
by hypothesis
\item\label{step:c31a:2} $(\forall\metavariable{x})\metavariable{R}\vdash(\forall\metavariable{x})\metavariable{R}\implies\metavariable{R}$
by \ref{c30}
\item\label{step:c31a:3} $(\forall\metavariable{x})\metavariable{R}\vdash(\forall\metavariable{x})\metavariable{R}$
by assumption
\item\label{step:c31a:4} $(\forall\metavariable{x})\metavariable{R}\vdash\metavariable{R}$
by MP(\ref{step:c31a:2}, \ref{step:c31a:3})
\item\label{step:c31a:5} $(\forall\metavariable{x})\metavariable{R}\vdash\metavariable{R}\implies\metavariable{S}$
by weakening \ref{step:c31a:1}
\item\label{step:c31a:6} $(\forall\metavariable{x})\metavariable{R}\vdash\metavariable{S}$
by MP(\ref{step:c31a:5}, \ref{step:c31a:4})
\item\label{step:c31a:7} $(\forall\metavariable{x})\metavariable{R}\vdash(\forall\metavariable{x})\metavariable{S}$
by \ref{c27}(\ref{step:c31a:6}, $\metavariable{x}$) 
\item\label{step:c31a:8} $\vdash(\forall\metavariable{x})\metavariable{R}\implies(\forall\metavariable{x})\metavariable{S}$
by \ref{c14}(\ref{step:c31a:7})
\end{pf}
\item
\begin{pf}
\item\label{step:c31b:1} $\vdash\metavariable{R}\implies\metavariable{S}$
by hypothesis
\item\label{step:c31b:2} $\vdash\neg\metavariable{S}\implies\neg\metavariable{R}$
by contrapositive of \ref{step:c31b:1}
\item\label{step:c31b:3} $\vdash(\forall\metavariable{x})\neg\metavariable{S}\implies(\forall\metavariable{x})\neg\metavariable{R}$
by applying (1) of this theorem to \ref{step:c31b:2}
\item\label{step:c31b:4} $\vdash\neg(\forall\metavariable{x})\neg\metavariable{R}\implies\neg(\forall\metavariable{x})\neg\metavariable{S}$
by contrapositive of \ref{step:c31b:3}, and using Bourbaki's definition
of $\forall$.
\end{pf}
\end{enumerate}

\subsubsection{Addendum} Observe that $\vdash(\forall\metavariable{x})\metavariable{R}\implies\metavariable{R}$
by \ref{c30}($\metavariable{R}$, $\metavariable{x}$, $\metavariable{x}$).

\begin{dc}\label{c32}%
Let $\metavariable{R}$ and $\metavariable{S}$ be relations in $\theory{T}$.
\begin{enumerate}
\item $\vdash(\forall\metavariable{x})(\metavariable{R}\land\metavariable{S})\iff\Bigl(\bigl((\forall\metavariable{x})\metavariable{R}\bigr)\land\bigl((\forall\metavariable{x})\metavariable{S}\bigr)\Bigr)$
\item $\vdash(\exists\metavariable{x})(\metavariable{R}\lor\metavariable{S})\iff\Bigl(\bigl((\exists\metavariable{x})\metavariable{R}\bigr)\lor\bigl((\exists\metavariable{x})\metavariable{S}\bigr)\Bigr)$
\end{enumerate}
\end{dc}
It suffices to prove (1), since (2) follows from (1) and \ref{c29}.
\begin{pf}
\item\label{step:c32:1}\Pf $(\forall\metavariable{x})(\metavariable{R}\land\metavariable{S})\vdash\metavariable{R}\land\metavariable{S}$
by \ref{c30}($\metavariable{R}$, $\metavariable{x}$, $\metavariable{x}$)
\item\label{step:c32:2} $(\forall\metavariable{x})(\metavariable{R}\land\metavariable{S})\vdash\metavariable{R}$
\item\label{step:c32:3} $(\forall\metavariable{x})(\metavariable{R}\land\metavariable{S})\vdash(\forall\metavariable{x})\metavariable{R}$
\item\label{step:c32:4} $(\forall\metavariable{x})(\metavariable{R}\land\metavariable{S})\vdash\metavariable{S}$
\item\label{step:c32:5} $(\forall\metavariable{x})(\metavariable{R}\land\metavariable{S})\vdash(\forall\metavariable{x})\metavariable{S}$
\item\label{step:c32:6} $(\forall\metavariable{x})(\metavariable{R}\land\metavariable{S})\vdash((\forall\metavariable{x})\metavariable{R})\land((\forall\metavariable{x})\metavariable{S})$
\item\label{step:c32:7} $\vdash(\forall\metavariable{x})(\metavariable{R}\land\metavariable{S})\implies((\forall\metavariable{x})\metavariable{R})\land((\forall\metavariable{x})\metavariable{S})$
by \ref{c14}(\ref{step:c32:6})
\item\label{step:c32:8} $(\forall\metavariable{x})\metavariable{R},(\forall\metavariable{x})\metavariable{S}\vdash(\forall\metavariable{x})\metavariable{R}$
by assumption
\item\label{step:c32:9} $(\forall\metavariable{x})\metavariable{R},(\forall\metavariable{x})\metavariable{S}\vdash(\forall\metavariable{x})\metavariable{R}\implies\metavariable{R}$
by \ref{c30}($\metavariable{R}$, $\metavariable{x}$, $\metavariable{x}$)
\item\label{step:c32:10} $(\forall\metavariable{x})\metavariable{R},(\forall\metavariable{x})\metavariable{S}\vdash\metavariable{R}$
by MP(\ref{step:c32:9}, \ref{step:c32:8})
\item\label{step:c32:11} $(\forall\metavariable{x})\metavariable{R},(\forall\metavariable{x})\metavariable{S}\vdash(\forall\metavariable{x})\metavariable{S}$
by assumption
\item\label{step:c32:12} $(\forall\metavariable{x})\metavariable{R},(\forall\metavariable{x})\metavariable{S}\vdash(\forall\metavariable{x})\metavariable{S}\implies\metavariable{S}$
by \ref{c30}($\metavariable{S}$, $\metavariable{x}$, $\metavariable{x}$)
\item\label{step:c32:13} $(\forall\metavariable{x})\metavariable{R},(\forall\metavariable{x})\metavariable{S}\vdash\metavariable{S}$
by MP(\ref{step:c32:12}, \ref{step:c32:11})
\item\label{step:c32:14} $(\forall\metavariable{x})\metavariable{R},(\forall\metavariable{x})\metavariable{S}\vdash\metavariable{R}\land\metavariable{S}$
by \ref{c20}(\ref{step:c32:10}, \ref{step:c32:13})
\item\label{step:c32:15} $(\forall\metavariable{x})\metavariable{R},(\forall\metavariable{x})\metavariable{S}\vdash(\forall\metavariable{x})(\metavariable{R}\land\metavariable{S})$
by \ref{c27}(\ref{step:c32:14}, $\metavariable{x}$)
\item\label{step:c32:16} $\vdash(\forall\metavariable{x})\metavariable{R}\land(\forall\metavariable{x})\metavariable{S}\implies(\forall\metavariable{x})(\metavariable{R}\land\metavariable{S})$
\end{pf}

\begin{dc}\label{c33}%
Let $\metavariable{R}$ and $\metavariable{S}$ be relations in $\theory{T}$.
Let $\metavariable{x}$ be a letter. Assume $\metavariable{x}$ does not
appear in $\metavariable{R}$.
\begin{enumerate}
\item $\vdash(\forall\metavariable{x})(\metavariable{R}\lor\metavariable{S})\iff\Bigl(\metavariable{R}\lor\bigl((\forall\metavariable{x})\metavariable{S}\bigr)\Bigr)$
\item $\vdash(\exists\metavariable{x})(\metavariable{R}\land\metavariable{S})\iff\Bigl(\metavariable{R}\land\bigl((\exists\metavariable{x})\metavariable{S}\bigr)\Bigr)$
\end{enumerate}
Note the use of disjunction and conjunction is paired with opposite
quantifiers as found in \ref{c32}.
\end{dc}
Observe (2) follows from (1) and \ref{c29}.

\begin{dc}\label{c34}%
Let $\metavariable{R}$ be a relation in $\theory{T}$.
\begin{enumerate}
\item $\vdash(\forall\metavariable{x})(\forall\metavariable{y})\metavariable{R}\iff(\forall\metavariable{y})(\forall\metavariable{x})\metavariable{R}$
\item $\vdash(\exists\metavariable{x})(\exists\metavariable{y})\metavariable{R}\iff(\exists\metavariable{y})(\exists\metavariable{x})\metavariable{R}$
\item $\vdash(\exists\metavariable{x})(\forall\metavariable{y})\metavariable{R}\implies(\forall\metavariable{y})(\exists\metavariable{x})\metavariable{R}$
\end{enumerate}
\end{dc}
